Stimpfle/eProds.thy
@@ -57,14 +57,14 @@ fun munge0 :: "('n, 't) prods \<Rightarrow> ('n, 't) syms \<Rightarrow> ('n, 't)
     if nullable P s then ((map ((#) s) (munge0 P sl)) @ munge0 P sl) 
     else (map ((#) s) (munge0 P sl)))"
 
-definition munge :: "('n, 't) prods \<Rightarrow> ('n, 't) prodS" where
+definition munge :: "('n, 't) prods \<Rightarrow> ('n, 't) Prods" where
 "munge P = {(l,r'). \<exists>r. (l,r) \<in> set P \<and> r' \<in> set (munge0 P r) \<and> (r' \<noteq> [])}"
 
 definition nepr :: "('n,'t) prods \<Rightarrow> ('n,'t) prods \<Rightarrow> bool" where 
   "nepr P P' = (set P' = munge P)"
 
 (* auxiliary function to prove finiteness *)
-definition munge_fun :: "('n, 't) prods \<Rightarrow> ('n, 't) prod \<Rightarrow> ('n, 't) prodS" where 
+definition munge_fun :: "('n, 't) prods \<Rightarrow> ('n, 't) prod \<Rightarrow> ('n, 't) Prods" where 
   "munge_fun P p = {(l',r'). l' = fst p \<and> r' \<in> set (munge0 P (snd p)) \<and> (r' \<noteq> [])}"
 
 lemma munge_fun_eq: "munge P = \<Union>((munge_fun P) ` set P)"
@@ -317,40 +317,40 @@ next
   qed
 qed
 
-(* Proof that Aditis definition of L G is the same as Lang (prodS G) (start G). This part has become obsolete *)
+(* Proof that Aditis definition of L G is the same as Lang (Prods G) (start G). This part has become obsolete *)
 definition "isWord w \<longleftrightarrow> (\<nexists>A. Nt A \<in> set w)"   
-definition "L G = {w. prodS G \<turnstile> [Nt (start G)] \<Rightarrow>* w \<and> isWord w}"
+definition "L G = {w. Prods G \<turnstile> [Nt (start G)] \<Rightarrow>* w \<and> isWord w}"
 
-lemma L_eq_Lang1: "(map Tm) ` Lang (prodS G) (start G) \<subseteq> L G"
+lemma L_eq_Lang1: "(map Tm) ` Lang (Prods G) (start G) \<subseteq> L G"
 proof -
-  have "\<forall>w \<in> Lang (prodS G) (start G). isWord (map Tm w)"
+  have "\<forall>w \<in> Lang (Prods G) (start G). isWord (map Tm w)"
     unfolding isWord_def by auto
-  moreover have "\<forall>w \<in> Lang (prodS G) (start G). (prodS G) \<turnstile> [Nt (start G)] \<Rightarrow>* (map Tm w)"
+  moreover have "\<forall>w \<in> Lang (Prods G) (start G). (Prods G) \<turnstile> [Nt (start G)] \<Rightarrow>* (map Tm w)"
     unfolding Lang_def by simp
   ultimately show ?thesis
     using L_def by blast
 qed
 
-lemma L_eq_Lang2: "L G \<subseteq> (map Tm) ` Lang (prodS G) (start G)"
+lemma L_eq_Lang2: "L G \<subseteq> (map Tm) ` Lang (Prods G) (start G)"
 proof 
   fix w
   assume "w \<in> L G"
-  hence 1: "prodS G \<turnstile> [Nt (start G)] \<Rightarrow>* w \<and> isWord w"
+  hence 1: "Prods G \<turnstile> [Nt (start G)] \<Rightarrow>* w \<and> isWord w"
     using L_def by blast
   obtain w' where "w = map Tm w'"
     by (metis 1 ex_map_conv isWord_def sym.exhaust)
-  hence "w' \<in> {w'. prodS G \<turnstile> [Nt (start G)] \<Rightarrow>* map Tm w'}"
+  hence "w' \<in> {w'. Prods G \<turnstile> [Nt (start G)] \<Rightarrow>* map Tm w'}"
     using 1 by blast
-  hence "w \<in> (map Tm) ` {w'. prodS G \<turnstile> [Nt (start G)] \<Rightarrow>* map Tm w'}"
+  hence "w \<in> (map Tm) ` {w'. Prods G \<turnstile> [Nt (start G)] \<Rightarrow>* map Tm w'}"
     using \<open>w = map Tm w'\<close> by blast
-  thus "w \<in> (map Tm) ` Lang (prodS G) (start G)"
+  thus "w \<in> (map Tm) ` Lang (Prods G) (start G)"
     by (simp add: Lang_def)
 qed
 
-lemma L_eq_Lang: "L G = (map Tm) ` Lang (prodS G) (start G)"
+lemma L_eq_Lang: "L G = (map Tm) ` Lang (Prods G) (start G)"
   using L_eq_Lang1 L_eq_Lang2 by blast
 
-lemma L_Lang: "L G = L G' \<longleftrightarrow> Lang (prodS G) (start G) = Lang (prodS G') (start G')"
+lemma L_Lang: "L G = L G' \<longleftrightarrow> Lang (Prods G) (start G) = Lang (Prods G') (start G')"
   using L_eq_Lang by (metis (mono_tags, lifting) Collect_cong L_def Lang_def image_eqI mem_Collect_eq)
 
 theorem nepr_eq_if_noe:
